Weidenbach_Book/IsaSAT_Propagate_Conflict.thy
@@ -316,11 +316,6 @@ sepref_thm update_clause_wl_code
     fmap_swap_ll_u64_def[symmetric]
     fmap_swap_ll_def[symmetric]
     PR_CONST_def
-    apply sepref_dbg_keep
-    apply sepref_dbg_trans_keep
-    apply sepref_dbg_trans_step_keep
-    oops
-    apply sepref_dbg_side_unfold apply (auto simp: )[]
   by sepref
 
 concrete_definition (in -) update_clause_wl_code
@@ -330,8 +325,8 @@ concrete_definition (in -) update_clause_wl_code
 prepare_code_thms (in -) update_clause_wl_code_def
 
 lemmas update_clause_wl_code[sepref_fr_rules] =
-  update_clause_wl_code.refine[OF isasat_input_bounded_nempty_axioms]
-
+  update_clause_wl_code.refine[OF isasat_input_bounded_nempty_axioms, unfolded PR_CONST_def]
+(* 
 thm update_clause_wl_code_pre_def
 sepref_thm update_clause_wl_fast_code
   is \<open>uncurry6 update_clause_wl_heur\<close>
@@ -356,20 +351,18 @@ concrete_definition (in -) update_clause_wl_fast_code
 prepare_code_thms (in -) update_clause_wl_fast_code_def
 
 lemmas update_clause_wl_fast_code[sepref_fr_rules] =
-  update_clause_wl_fast_code.refine[OF isasat_input_bounded_nempty_axioms]
+  update_clause_wl_fast_code.refine[OF isasat_input_bounded_nempty_axioms] *)
 
+sepref_register propagate_lit_wl_heur
 sepref_thm propagate_lit_wl_code
-  is \<open>uncurry3 (RETURN oooo (PR_CONST propagate_lit_wl_heur))\<close>
+  is \<open>uncurry3 (PR_CONST propagate_lit_wl_heur)\<close>
   :: \<open>[propagate_lit_wl_heur_pre]\<^sub>a
-      unat_lit_assn\<^sup>k *\<^sub>a nat_assn\<^sup>k *\<^sub>a uint64_nat_assn\<^sup>k *\<^sub>a isasat_assn\<^sup>d \<rightarrow> isasat_assn\<close>
+      unat_lit_assn\<^sup>k *\<^sub>a nat_assn\<^sup>k *\<^sub>a nat_assn\<^sup>k *\<^sub>a isasat_assn\<^sup>d \<rightarrow> isasat_assn\<close>
   unfolding PR_CONST_def propagate_lit_wl_heur_def isasat_assn_def
     cons_trail_Propagated_def[symmetric]
   supply [[goals_limit=1]]length_rll_def[simp] length_ll_def[simp]
   unfolding update_clause_wl_heur_def isasat_assn_def
     propagate_lit_wl_heur_pre_def fmap_swap_ll_def[symmetric]
-    fmap_swap_ll_u64_def[symmetric]
-    zero_uint64_nat_def[symmetric]
-    one_uint64_nat_def[symmetric]
   by sepref
 
 
@@ -382,7 +375,7 @@ prepare_code_thms (in -) propagate_lit_wl_code_def
 lemmas propagate_lit_wl_code[sepref_fr_rules] =
   propagate_lit_wl_code.refine[OF isasat_input_bounded_nempty_axioms, unfolded PR_CONST_def]
 
-sepref_thm propagate_lit_wl_fast_code
+(* sepref_thm propagate_lit_wl_fast_code
   is \<open>uncurry3 (RETURN oooo (PR_CONST propagate_lit_wl_heur))\<close>
   :: \<open>[\<lambda>(((L', C), w), S). propagate_lit_wl_heur_pre (((L', C), w), S) \<and>
         w + 1 \<le> uint64_max]\<^sub>a
@@ -405,9 +398,9 @@ concrete_definition (in -) propagate_lit_wl_fast_code
 prepare_code_thms (in -) propagate_lit_wl_fast_code_def
 
 lemmas propagate_lit_wl_fast_code[sepref_fr_rules] =
-  propagate_lit_wl_fast_code.refine[OF isasat_input_bounded_nempty_axioms, unfolded PR_CONST_def]
+  propagate_lit_wl_fast_code.refine[OF isasat_input_bounded_nempty_axioms, unfolded PR_CONST_def] *)
 
-
+sepref_register keep_watch_heur
 sepref_thm keep_watch_heur
   is \<open>uncurry3 (PR_CONST keep_watch_heur)\<close>
   :: \<open>unat_lit_assn\<^sup>k *\<^sub>a nat_assn\<^sup>k *\<^sub>a nat_assn\<^sup>k *\<^sub>a isasat_assn\<^sup>d \<rightarrow>\<^sub>a isasat_assn\<close>
@@ -436,11 +429,50 @@ prepare_code_thms (in -) keep_watch_heur_code_def
 lemmas keep_watch_heur_code[sepref_fr_rules] =
   keep_watch_heur_code.refine[OF isasat_input_bounded_nempty_axioms, unfolded PR_CONST_def]
 
+lemma clause_not_marked_to_delete_heur_alt_def:
+  \<open>RETURN \<circ>\<circ> clause_not_marked_to_delete_heur = (\<lambda>(M, arena, D, oth) C.
+     RETURN (arena_status arena C \<noteq> DELETED))\<close>
+  unfolding clause_not_marked_to_delete_heur_def by (auto intro!: ext)
 
+(* TODO Move *)
+lemma (in-) nat_of_uint32_Suc03_iff:
+ \<open>nat_of_uint32 a = Suc 0 \<longleftrightarrow> a = 1\<close>
+   \<open>nat_of_uint32 a = 3 \<longleftrightarrow> a = 3\<close>
+   using word_nat_of_uint32_Rep_inject nat_of_uint32_3 by fastforce+
+lemma  (in -) nat_of_uint32_013_neq:
+  "(1::uint32) \<noteq> (0 :: uint32)" "(0::uint32) \<noteq> (1 :: uint32)"
+  "(3::uint32) \<noteq> (0 :: uint32)"
+  "(3::uint32) \<noteq> (1 :: uint32)"
+  "(0::uint32) \<noteq> (3 :: uint32)"
+  "(1::uint32) \<noteq> (3 :: uint32)"
+  by (auto dest: arg_cong[of _ _ nat_of_uint32] simp: nat_of_uint32_3)
+
+lemma (in -) status_assn_hnr_eq[sepref_fr_rules]:
+  \<open>(uncurry (return oo (=)), uncurry (RETURN oo (=))) \<in> status_assn\<^sup>k *\<^sub>a status_assn\<^sup>k \<rightarrow>\<^sub>a
+    bool_assn\<close>
+  by sepref_to_hoare (sep_auto simp: status_rel_def hr_comp_def uint32_nat_rel_def br_def
+    nat_of_uint32_0_iff nat_of_uint32_Suc03_iff nat_of_uint32_013_neq)
+find_theorems INIT status_assn
+lemma INIT_status_assn[sepref_fr_rules]:
+  \<open>(uncurry0 (return 0), uncurry0 (RETURN INIT)) \<in> unit_assn\<^sup>k \<rightarrow>\<^sub>a status_assn\<close>
+  by (sepref_to_hoare) (sep_auto simp: status_rel_def hr_comp_def uint32_nat_rel_def br_def)
+
+lemma LEARNED_status_assn[sepref_fr_rules]:
+  \<open>(uncurry0 (return 1), uncurry0 (RETURN LEARNED)) \<in> unit_assn\<^sup>k \<rightarrow>\<^sub>a status_assn\<close>
+  by (sepref_to_hoare) (sep_auto simp: status_rel_def hr_comp_def uint32_nat_rel_def br_def)
+
+lemma DELETED_status_assn[sepref_fr_rules]:
+  \<open>(uncurry0 (return 3), uncurry0 (RETURN DELETED)) \<in> unit_assn\<^sup>k \<rightarrow>\<^sub>a status_assn\<close>
+  by (sepref_to_hoare) (sep_auto simp: status_rel_def hr_comp_def uint32_nat_rel_def br_def
+    nat_of_uint32_Suc03_iff)
+
+(* End Move *)
 sepref_thm clause_not_marked_to_delete_heur_code
   is \<open>uncurry (RETURN oo clause_not_marked_to_delete_heur)\<close>
-  :: \<open>isasat_assn\<^sup>k *\<^sub>a nat_assn\<^sup>k \<rightarrow>\<^sub>a bool_assn\<close>
-  unfolding clause_not_marked_to_delete_heur_def
+  :: \<open>[clause_not_marked_to_delete_heur_pre]\<^sub>a isasat_assn\<^sup>k *\<^sub>a nat_assn\<^sup>k \<rightarrow> bool_assn\<close>
+  supply [[goals_limit=1]]
+  unfolding clause_not_marked_to_delete_heur_alt_def isasat_assn_def
+     clause_not_marked_to_delete_heur_pre_def
   by sepref
 
 concrete_definition (in -) clause_not_marked_to_delete_heur_code
@@ -451,8 +483,7 @@ prepare_code_thms (in -) clause_not_marked_to_delete_heur_code_def
 
 lemmas clause_not_marked_to_delete_heur_refine[sepref_fr_rules] =
    clause_not_marked_to_delete_heur_code.refine[of \<A>\<^sub>i\<^sub>n, OF isasat_input_bounded_nempty_axioms]
-find_theorems arrayO_assn update_ll
-thm update_blit_wl_heur_def
+
 sepref_thm update_blit_wl_heur_code
   is \<open>uncurry5 update_blit_wl_heur\<close>
   :: \<open>unat_lit_assn\<^sup>k *\<^sub>a nat_assn\<^sup>k *\<^sub>a nat_assn\<^sup>k *\<^sub>a nat_assn\<^sup>k *\<^sub>a unat_lit_assn\<^sup>k *\<^sub>a isasat_assn\<^sup>d \<rightarrow>\<^sub>a 
@@ -481,10 +512,8 @@ begin
 
 context
 begin
+find_theorems keep_watch_heur
 
-thm unit_propagation_inner_loop_wl_loop_D_heur_inv0_def unit_propagation_inner_loop_wl_loop_D_inv_def
-unit_prop_body_wl_heur_inv_def
-sepref_register find_unwatched_wl_st_heur
 sepref_thm unit_propagation_inner_loop_body_wl_heur
   is \<open>uncurry3 (PR_CONST unit_propagation_inner_loop_body_wl_heur)\<close>
   :: \<open>unat_lit_assn\<^sup>k *\<^sub>a nat_assn\<^sup>k *\<^sub>a nat_assn\<^sup>k *\<^sub>a isasat_assn\<^sup>d \<rightarrow>\<^sub>a nat_assn *a nat_assn *a isasat_assn\<close>
@@ -502,8 +531,6 @@ sepref_thm unit_propagation_inner_loop_body_wl_heur
   unfolding fmap_rll_def[symmetric]
   unfolding fast_minus_def[symmetric]
     SET_FALSE_def[symmetric] SET_TRUE_def[symmetric]
-  apply (rewrite in \<open>let _ = \<hole> in _\<close> zero_uint64_nat_def[symmetric])+
-  apply (rewrite in \<open>let _ = \<hole> in _\<close> one_uint64_nat_def[symmetric])+
   by sepref
 
 (* sepref_thm unit_propagation_inner_loop_body_wl_fast_heur
@@ -586,7 +613,6 @@ prepare_code_thms (in -) length_ll_fs_heur_code_def
 lemmas length_ll_fs_heur_code_refine[sepref_fr_rules] =
    length_ll_fs_heur_code.refine[of \<A>\<^sub>i\<^sub>n, OF isasat_input_bounded_nempty_axioms]
 
-term length_aa_u32
 sepref_thm length_ll_fs_heur_fast_code
   is \<open>uncurry (RETURN oo length_ll_fs_heur)\<close>
   :: \<open>[\<lambda>(S, L). nat_of_lit L < length (get_watched_wl_heur S) \<and>
@@ -756,7 +782,7 @@ sepref_thm cut_watch_list_heur2
   unfolding cut_watch_list_heur2_def isasat_assn_def length_ll_def[symmetric]
   update_ll_def[symmetric] nth_rll_def[symmetric] shorten_take_ll_def[symmetric]
   by sepref
- 
+
 concrete_definition (in -) cut_watch_list_heur2_code
    uses isasat_input_bounded_nempty.cut_watch_list_heur2.refine_raw
    is \<open>(uncurry3 ?f, _)\<in>_\<close>
@@ -815,14 +841,14 @@ definition get_literals_to_update_wl_heur_W_list where
 definition literals_to_update_wl_empty_heur' :: \<open>twl_st_wl_heur_W_list \<Rightarrow> bool\<close>  where
   \<open>literals_to_update_wl_empty_heur' = (\<lambda>(M, N, D, Q, W, oth). Q = [])\<close>
 
-
+thm isasat_assn_def
 definition (in isasat_input_ops) twl_st_wl_heur_W_list_rel
   :: \<open>(twl_st_wl_heur_W_list \<times> twl_st_wl_heur) set\<close>
 where
   \<open>twl_st_wl_heur_W_list_rel =
      (Id :: ((nat,nat) ann_lits \<times> _) set) \<times>\<^sub>r
-     (Id :: (nat clauses_l  \<times> _) set) \<times>\<^sub>r
-     (Id :: (nat cconflict \<times> _)set) \<times>\<^sub>r
+     (Id :: (arena  \<times> _) set) \<times>\<^sub>r
+     (Id :: (conflict_option_rel \<times> _)set) \<times>\<^sub>r
      (list_mset_rel :: (nat literal list \<times> nat lit_queue_wl) set)  \<times>\<^sub>r
      (Id :: ((nat watcher) list list \<times> _)set) \<times>\<^sub>r
      Id \<times>\<^sub>r
@@ -842,10 +868,10 @@ definition (in isasat_input_ops) twl_st_heur_W_list_assn
   :: \<open>twl_st_wl_heur_W_list \<Rightarrow> twl_st_wll_trail \<Rightarrow> assn\<close>
 where
 \<open>twl_st_heur_W_list_assn =
-  trail_assn *a clauses_ll_assn *a
-  option_lookup_clause_assn *a
+  trail_assn *a arena_assn *a
+  isasat_conflict_assn *a
   (list_assn unat_lit_assn) *a
-  arrayO_assn (arl_assn (nat_assn *a unat_lit_assn)) *a
+  watchlist_assn *a
   vmtf_remove_conc *a phase_saver_conc *a uint32_nat_assn *a cach_refinement_assn *a
   lbd_assn *a out_learned_assn *a stats_assn *a ema_assn *a ema_assn *a
   conflict_count_assn *a vdom_assn *a nat_assn
@@ -856,7 +882,7 @@ lemma (in isasat_input_ops) isasat_assn_W_list:
   unfolding isasat_assn_def twl_st_heur_W_list_assn_def twl_st_wl_heur_W_list_rel_def
   by (auto simp: list_assn_list_mset_rel_eq_list_mset_assn)
 
-
+(* 
 definition (in isasat_input_ops) twl_st_heur_W_list_fast_assn
   :: \<open>_ \<Rightarrow> twl_st_wll_trail_fast \<Rightarrow> assn\<close>
 where
@@ -873,7 +899,7 @@ where
 lemma (in isasat_input_ops) isasat_fast_assn_W_list:
   \<open>isasat_fast_assn = hr_comp twl_st_heur_W_list_fast_assn twl_st_wl_heur_W_list_rel\<close>
   unfolding isasat_fast_assn_def twl_st_heur_W_list_fast_assn_def twl_st_wl_heur_W_list_rel_def
-  by (auto simp: list_assn_list_mset_rel_eq_list_mset_assn)
+  by (auto simp: list_assn_list_mset_rel_eq_list_mset_assn) *)
 
 sepref_thm select_and_remove_from_literals_to_update_wl_code
   is \<open>RETURN o select_and_remove_from_literals_to_update_wl_heur'\<close>
@@ -884,7 +910,6 @@ sepref_thm select_and_remove_from_literals_to_update_wl_code
     literals_to_update_wl_empty_heur'_def
   supply [[goals_limit = 1]]
   by sepref
-
 
 concrete_definition (in -) select_and_remove_from_literals_to_update_wl_code
    uses isasat_input_bounded_nempty.select_and_remove_from_literals_to_update_wl_code.refine_raw
@@ -897,7 +922,7 @@ lemmas select_and_remove_from_literals_to_update_wl_code_refine[sepref_fr_rules]
      OF isasat_input_bounded_nempty_axioms]
 
 
-sepref_thm select_and_remove_from_literals_to_update_wl_fast_code
+(* sepref_thm select_and_remove_from_literals_to_update_wl_fast_code
   is \<open>RETURN o select_and_remove_from_literals_to_update_wl_heur'\<close>
   :: \<open>[\<lambda>S. \<not>literals_to_update_wl_empty_heur' S]\<^sub>a
       twl_st_heur_W_list_fast_assn\<^sup>d \<rightarrow> twl_st_heur_W_list_fast_assn *a unat_lit_assn\<close>
@@ -915,7 +940,7 @@ prepare_code_thms (in -) select_and_remove_from_literals_to_update_wl_fast_code_
 
 lemmas select_and_remove_from_literals_to_update_wl_fast_code_refine[sepref_fr_rules] =
    select_and_remove_from_literals_to_update_wl_fast_code.refine[of \<A>\<^sub>i\<^sub>n,
-     OF isasat_input_bounded_nempty_axioms]
+     OF isasat_input_bounded_nempty_axioms] *)
 
 definition (in -)literals_to_update_wl_empty_heur :: \<open>twl_st_wl_heur \<Rightarrow> bool\<close>  where
   \<open>literals_to_update_wl_empty_heur S \<longleftrightarrow> literals_to_update_wl_heur S = {#}\<close>
@@ -947,14 +972,14 @@ theorem
      select_and_remove_from_literals_to_update_wl_heur)
     \<in> [\<lambda>S. \<not> literals_to_update_wl_empty_heur S]\<^sub>a isasat_assn\<^sup>d \<rightarrow> isasat_assn *a
           unat_lit_assn\<close>
-    (is ?slow is \<open>?fun \<in> [?pre]\<^sub>a ?im \<rightarrow> ?f\<close>) and
-  select_and_remove_from_literals_to_update_wl_fast_code_select_and_remove_from_literals_to_update_wl
+    (is ?slow is \<open>?fun \<in> [?pre]\<^sub>a ?im \<rightarrow> ?f\<close>)
+  (* select_and_remove_from_literals_to_update_wl_fast_code_select_and_remove_from_literals_to_update_wl
   [sepref_fr_rules]:
   \<open>(select_and_remove_from_literals_to_update_wl_fast_code,
      select_and_remove_from_literals_to_update_wl_heur)
     \<in> [\<lambda>S. \<not> literals_to_update_wl_empty_heur S]\<^sub>a isasat_fast_assn\<^sup>d \<rightarrow> isasat_fast_assn *a
           unat_lit_assn\<close>
-    (is ?fast is \<open>?cfast \<in> [?pre]\<^sub>a ?imfast \<rightarrow> ?ffast\<close>)
+    (is ?fast is \<open>?cfast \<in> [?pre]\<^sub>a ?imfast \<rightarrow> ?ffast\<close>) *)
 proof -
   have H: \<open>?fun
     \<in> [comp_PRE twl_st_wl_heur_W_list_rel (\<lambda>S. \<not> literals_to_update_wl_empty_heur S)
@@ -985,7 +1010,7 @@ proof -
      defer
     using H unfolding im f PR_CONST_def apply assumption
     using pre ..
-  have H: \<open>?cfast
+  (* have H: \<open>?cfast
     \<in> [comp_PRE twl_st_wl_heur_W_list_rel (\<lambda>S. \<not> literals_to_update_wl_empty_heur S)
      (\<lambda>_ S. \<not> literals_to_update_wl_empty_heur' S)
      (\<lambda>_. True)]\<^sub>a hrp_comp (twl_st_heur_W_list_fast_assn\<^sup>d)
@@ -1008,7 +1033,7 @@ proof -
     apply (rule hfref_weaken_pre[OF ])
      defer
     using H unfolding im f PR_CONST_def apply assumption
-    using pre ..
+    using pre .. *)
 qed
 
 sepref_thm literals_to_update_wl_empty_heur_code
@@ -1030,7 +1055,7 @@ lemmas literals_to_update_wl_empty_heur_code_refine[sepref_fr_rules] =
    literals_to_update_wl_empty_heur_code.refine[of \<A>\<^sub>i\<^sub>n, OF isasat_input_bounded_nempty_axioms]
 
 
-sepref_thm literals_to_update_wl_empty_heur_fast_code
+(* sepref_thm literals_to_update_wl_empty_heur_fast_code
   is \<open>RETURN o literals_to_update_wl_empty_heur'\<close>
   :: \<open>twl_st_heur_W_list_fast_assn\<^sup>k \<rightarrow>\<^sub>a bool_assn\<close>
   supply [[goals_limit=1]]
@@ -1047,7 +1072,7 @@ prepare_code_thms (in -) literals_to_update_wl_empty_heur_fast_code_def
 
 lemmas literals_to_update_wl_empty_heur_fast_code_refine[sepref_fr_rules] =
    literals_to_update_wl_empty_heur_fast_code.refine[of \<A>\<^sub>i\<^sub>n, OF isasat_input_bounded_nempty_axioms]
-
+*)
 lemma literals_to_update_wl_empty_heur_literals_to_update_wl_empty:
   \<open>(RETURN o literals_to_update_wl_empty_heur', RETURN o literals_to_update_wl_empty_heur) \<in>
     twl_st_wl_heur_W_list_rel \<rightarrow>\<^sub>f \<langle>Id\<rangle>nres_rel\<close>
@@ -1066,14 +1091,14 @@ lemma literals_to_update_wl_empty_heur_code_literals_to_update_wl_empty[sepref_f
   unfolding isasat_assn_W_list[symmetric]
   .
 
-
+(* 
 lemma literals_to_update_wl_empty_heur_fast_code_literals_to_update_wl_empty[sepref_fr_rules]:
   \<open>(literals_to_update_wl_empty_heur_fast_code, RETURN \<circ> literals_to_update_wl_empty_heur)
      \<in> isasat_fast_assn\<^sup>k \<rightarrow>\<^sub>a bool_assn\<close>
   using literals_to_update_wl_empty_heur_fast_code_refine[FCOMP
       literals_to_update_wl_empty_heur_literals_to_update_wl_empty]
   unfolding isasat_fast_assn_W_list[symmetric]
-  .
+  . *)
 
 lemma literals_to_update_wl_literals_to_update_wl_empty:
   \<open>literals_to_update_wl_heur S = {#} \<longleftrightarrow> literals_to_update_wl_empty_heur S\<close>
@@ -1100,7 +1125,7 @@ prepare_code_thms (in -) unit_propagation_outer_loop_wl_D_def
 lemmas unit_propagation_outer_loop_wl_D[sepref_fr_rules] =
    unit_propagation_outer_loop_wl_D.refine[of \<A>\<^sub>i\<^sub>n, OF isasat_input_bounded_nempty_axioms]
 
-lemma unit_propagation_outer_loop_wl_D_fast_still_fast:
+(* lemma unit_propagation_outer_loop_wl_D_fast_still_fast:
   assumes
     fast: \<open>\<forall>L\<in>#dom_m (get_clauses_wl_heur x). L < uint_max\<close> and
     inv: \<open>unit_propagation_outer_loop_wl_D_heur_inv x s'\<close> and
@@ -1112,7 +1137,7 @@ proof -
     using le fast L inv by (cases s')
       (auto simp: select_and_remove_from_literals_to_update_wl_heur_def
       unit_propagation_outer_loop_wl_D_heur_inv_def)
-qed
+qed *)
 
 (* 
 sepref_thm unit_propagation_outer_loop_wl_D_fast
